start proof
symbol_reserved is trivial; working on initial state simulation.

Seccomp.v
@@ -1,4 +1,5 @@
 Require Import compcert.common.AST.
+Require Import compcert.common.Events.
 Require Import compcert.common.Globalenvs.
 Require Import compcert.lib.Coqlib.
 Require Import compcert.lib.Integers.
@@ -98,3 +99,89 @@ Definition program := AST.program fundef type.
 Definition genv := Genv.t fundef type.
 
 End PROGRAM.
+
+Inductive state : Type :=
+  | State:
+    forall (a: int)              (** accumulator *)
+           (x: int)              (** index register *)
+           (m: ZMap.t int)       (** scratch memory *)
+           (f: function)         (** current function *)
+           (pc: Z),              (** program counter *)
+    state
+  | Callstate:
+    forall (fd: fundef),         (** calling function *)
+    state
+  | Returnstate:
+    forall (v: int),             (** local return value *)
+    state
+  .
+
+Section SEMANTICS.
+
+Definition instruction_at (f: function) (pc: Z) :=
+  list_nth_z f pc.
+
+Inductive step (ge: genv) : state -> trace -> state -> Prop :=
+  | exec_Salu_add_k:
+      forall a x m f pc k,
+      instruction_at f pc = Some (Salu_add_k k) ->
+      let a' := Int.add a k in
+      let pc' := pc + 1 in
+      step ge (State a x m f pc)
+        E0 (State a' x m f pc')
+  | exec_Salu_add_x:
+      forall a x m f pc,
+      instruction_at f pc = Some (Salu_add_x) ->
+      let a' := Int.add a x in
+      let pc' := pc + 1 in
+      step ge (State a x m f pc)
+        E0 (State a' x m f pc')
+(*
+  | exec_Sld_w_abs:
+      forall a a' x m f pc k,
+      instruction_at f pc = Some (Sld_w_abs k) ->
+      seccomp_bpf_load k a' ->
+      let pc' := pc + 1 in
+      step ge (State a x m f pc)
+        E0 (State a' x m f pc')
+*)
+  | exec_Sld_w_len:
+      forall a x m f pc,
+      instruction_at f pc = Some (Sld_w_len) ->
+      let pc' := pc + 1 in
+      step ge (State a x m f pc)
+        E0 (State sizeof_seccomp_data x m f pc')
+  | exec_Sldx_w_len:
+      forall a x m f pc,
+      instruction_at f pc = Some (Sld_w_len) ->
+      let pc' := pc + 1 in
+      step ge (State a x m f pc)
+        E0 (State a sizeof_seccomp_data m f pc')
+  | exec_Sret_k:
+      forall a x m f pc k,
+      instruction_at f pc = Some (Sret_k k) ->
+      step ge (State a x m f pc)
+        E0 (Returnstate k)
+  | exec_Sret_a:
+      forall a x m f pc,
+      instruction_at f pc = Some (Sret_a) ->
+      step ge (State a x m f pc)
+        E0 (Returnstate a)
+  | exec_call:
+      forall f,
+      step ge (Callstate (Internal f))
+        E0 (State Int.zero Int.zero (ZMap.init Int.zero) f 0)
+  .
+
+Inductive initial_state (p: program): state -> Prop :=
+  | initial_state_intro: forall b f,
+    let ge := Genv.globalenv p in
+    Genv.find_symbol ge p.(prog_main) = Some b ->
+    Genv.find_funct_ptr ge b = Some f ->
+    initial_state p (Callstate f).
+
+Inductive final_state: state -> int -> Prop :=
+  | final_state_intro: forall v,
+      final_state (Returnstate v) v.
+
+End SEMANTICS.
