Seccompspec.v
@@ -1,93 +1,20 @@
-Require Import compcert.common.Smallstep.
+Require Import compcert.common.AST.
 Require Import compcert.common.Events.
 Require Import compcert.common.Globalenvs.
+Require Import compcert.common.Smallstep.
+Require Import compcert.lib.Coqlib.
+Require Import compcert.lib.Integers.
+Require Import compcert.lib.Maps.
 Require Import Seccomp.
 
-Inductive state : Type :=
-  | State:
-    forall (a: int)              (** accumulator *)
-           (x: int)              (** index register *)
-           (m: ZMap.t int)       (** scratch memory *)
-           (f: function)         (** current function *)
-           (pc: Z),              (** program counter *)
-    state
-  | Callstate:
-    forall (f: function),        (** calling function *)
-    state
-  | Returnstate:
-    forall (v: int),             (** local return value *)
-    state
-  .
-
-Section RELSEM.
+Section SEMANTICS.
 
 (** access struct seccomp_data *)
 Variable seccomp_bpf_load : int -> int -> Prop.
 
-Variable ge: genv.
+(* Variable ge: genv. *)
 
-Definition instruction_at (f: function) (pc: Z) :=
-  list_nth_z f pc.
-
-Inductive step : state -> trace -> state -> Prop :=
-  | exec_Salu_add_k:
-      forall a x m f pc k,
-      instruction_at f pc = Some (Salu_add_k k) ->
-      let a' := Int.add a k in
-      let pc' := pc + 1 in
-      step (State a x m f pc)
-        E0 (State a' x m f pc')
-  | exec_Salu_add_x:
-      forall a x m f pc,
-      instruction_at f pc = Some (Salu_add_x) ->
-      let a' := Int.add a x in
-      let pc' := pc + 1 in
-      step (State a x m f pc)
-        E0 (State a' x m f pc')
-  | exec_Sld_w_abs:
-      forall a x m f pc k,
-      instruction_at f pc = Some (Sld_w_abs k) ->
-      seccomp_bpf_load k a' ->
-      let pc' := pc + 1 in
-      step (State a x m f pc)
-        E0 (State a' x m f pc')
-  | exec_Sld_w_len:
-      forall a x m f pc,
-      instruction_at f pc = Some (Sld_w_len) ->
-      let pc' := pc + 1 in
-      step (State a x m f pc)
-        E0 (State sizeof_seccomp_data x m f pc')
-  | exec_Sldx_w_len:
-      forall a x m f pc,
-      instruction_at f pc = Some (Sld_w_len) ->
-      let pc' := pc + 1 in
-      step (State a x m f pc)
-        E0 (State a sizeof_seccomp_data m f pc')
-  | exec_Sret_k:
-      forall a x m f pc k,
-      instruction_at f pc = Some (Sret_k k) ->
-      step (State a x m f pc)
-        E0 (Returnstate k)
-  | exec_Sret_a:
-      forall a x m f pc,
-      instruction_at f pc = Some (Sret_a) ->
-      step (State a x m f pc)
-        E0 (Returnstate a)
-  | exec_call:
-      forall f,
-      step (Callstate f)
-        E0 (State Int.zero Int.zero (ZMap.init Int.zero) f 0)
-  .
-
-End RELSEM.
-
-Inductive initial_state (p: program): state -> Prop :=
-  | initial_state_intro:
-      initial_state p (Callstate p.(prog_main)).
-
-Inductive final_state: state -> int -> Prop :=
-  | final_state_intro: forall v,
-      final_state (Returnstate v) v.
+End SEMANTICS.
 
 Definition semantics (p: program) :=
   Semantics step (initial_state p) final_state (Genv.globalenv p).
