Seccompproof.v
@@ -1,0 +1,47 @@
+Require Import compcert.cfrontend.Clight.
+Require Import compcert.common.AST.
+Require Import compcert.common.Errors.
+Require Import compcert.common.Globalenvs.
+Require Import compcert.common.Values.
+Require Import Seccomp.
+Require Import Seccompjit.
+
+Section PRESERVATION.
+
+Variable prog: Seccomp.program.
+Variable tprog: Clight.program.
+Hypothesis TRANSF: transf_program prog = OK tprog.
+Let ge := Genv.globalenv prog.
+Let tge := Genv.globalenv tprog.
+
+Lemma symbols_preserved:
+  forall (s: ident), Genv.find_symbol tge s = Genv.find_symbol ge s.
+Proof.
+  exact (Genv.find_symbol_transf_partial _ _ TRANSF).
+Qed.
+
+Inductive match_states: Seccomp.state -> Clight.state -> Prop :=
+  | match_state:
+      forall a x m f pc tf s k e le tm,
+      match_states (Seccomp.State a x m f pc)
+                   (Clight.State tf s k e le tm)
+  | match_callstate:
+      forall f tf args k tm
+        (TF: transf_fundef f = OK tf)
+        ,
+      match_states (Seccomp.Callstate f)
+                   (Clight.Callstate tf args k tm)
+  | match_returnstate:
+      forall v tv k tm
+        (MV: Vint v = tv),
+      match_states (Seccomp.Returnstate v)
+                   (Clight.Returnstate tv k tm)
+  .
+
+(*
+Lemma transf_initial_states:
+  forall S, Seccomp.initial_state prog S ->
+  exists R, Clight.initial_state tprog R /\ match_states S R.
+*)
+
+End PRESERVATION.
